\documentclass{exam}
\usepackage{amssymb,amsmath}
\begin{document}
	\textbf{5. b} (DeMorgan's is done incorrectly)\\
	
	\textbf{6. a} This is material implication.\\
	
	\textbf{7. }
	
	\begin{tabular}{cc|cccc|c}
		p&q&$p \leftrightarrow q$&$\neg(p \leftrightarrow q)$&$\neg q$&$p \leftrightarrow \neg q$&Conclusion\\
		\hline
		T&T&T&F&F&F&T\\
		T&F&F&T&T&T&T\\
		F&T&F&T&F&T&T\\
		F&F&T&F&T&F&T\\
	\end{tabular}

	Conclusion: Since the two columns $\neg(p \leftrightarrow q)$ and $p \leftrightarrow \neg q$ are identical, $\neg(p \leftrightarrow q) \equiv p \leftrightarrow \neg q$.\\
	
	\textbf{8.}
	
	\begin{tabular}{c|c|c}
		Step&Statement&Rule\\
		\hline
		5&$p \rightarrow r$&contrapositive of 2.\\
		6&$p$&disjunctive syllogism (4. and 1.)\\
		7&$r$&modus ponens (6. and 5.)\\
		8&$s$&modus ponens (3. and 7.)\\
	\end{tabular}

	$\therefore$ Using the rules of inference and premises, we have shown $s$.\\
	
	\textbf{9.} $\forall y \exists x_1 \exists x_2 ( M(y) \rightarrow ( (T(x_1, y) \wedge C(x_1)) \wedge (T(x_2, y) \wedge F(x_2))  ))$\\
	
	\textbf{10.} $\forall x \exists y (F(x) \rightarrow (T(x,y) \wedge M(y)))$\\
	
	\textbf{11.} $\exists x (F(x) \wedge C(x))$\\
	
	\textbf{12.} $\exists x_1 \exists x_2  \forall x_3 ( C(x_1) \wedge C(x_2) \wedge (x_1 \neq x_2) \wedge ((x_1 \neq x_3) \wedge (x_2 \neq x_3)) \rightarrow \neg C(x_3))$
	
	
	
	
\end{document}